Aneris adequacy multiple (#32)
- Improved Trillium adequacy definition for multiple threads
- Added Aneris adequacy theorems for multiple threads/nodes

aneris/aneris_lang/program_logic/aneris_adequacy.v
@@ -3,6 +3,153 @@ From aneris.aneris_lang Require Import network adequacy.
 From aneris.aneris_lang.program_logic Require Export aneris_weakestpre.
 From aneris.algebra Require Import disj_gsets.
 
+Notation aneris_wptp ts Φs :=
+  ([∗ list] t;Φ ∈ ts;Φs, WP (expr_e t) @[expr_n t] ⊤ {{ Φ }})%I.
+
+Definition aneris_adequate_multiple
+           (es : list aneris_expr) (σ : state) (φs : list (val → Prop))  :=
+  adequate_multiple
+    NotStuck es σ
+    ((λ φ v _, φ v) <$>
+     ((λ eφ, λ v, ∃ w, v = mkVal (expr_n eφ.1) w ∧ eφ.2 w) <$> (zip es φs))).
+
+Lemma big_sepL_prefixes_l {PROP:bi} {X Y}
+      (xs xs' : list X) (ys : list Y) (Φ : X → Y → PROP) :
+  ([∗ list] x;y ∈ xs;ys, Φ x y) -∗
+  ([∗ list] x;y ∈ prefixes_from xs' xs;ys, Φ x.2 y).
+Proof.
+  iIntros "HΦs".
+  iInduction xs as [|x xs] "IHxs" forall (ys xs'); [done|].
+  destruct ys; [done|]=> /=.
+  iDestruct "HΦs" as "[$ HΦs]".
+  by iApply "IHxs".
+Qed.
+
+Theorem adequacy_multiple_strong Σ Mdl `{anerisPreG Σ Mdl} `{EqDecision (aneris_to_trace_model Mdl)}
+        A lbls obs_send_sas obs_rec_sas (es : list aneris_expr) σ (φs : list (val → Prop)) :
+  length es >= 1 →
+  aneris_model_rel_finitary Mdl →
+  (∀ (aG : anerisG Mdl Σ), ⊢ |={⊤}=>
+     unallocated A -∗
+     ([∗ set] sa ∈ A, sa ⤳[bool_decide (sa ∈ obs_send_sas),
+                           bool_decide (sa ∈ obs_rec_sas)] (∅, ∅)) -∗
+     ([∗ set] ip ∈ get_ips es,
+        ([∗ map] l ↦ v ∈ (state_heaps σ !!! ip), l ↦[ip] v) ∗
+        ([∗ map] sh ↦ s ∈ (state_sockets σ !!! ip), sh ↪[ip] s.1)) -∗
+     ([∗ map] ip ↦ ports ∈ (addrs_to_ip_ports_map
+                              (A ∖ (ports_in_use $ state_sockets σ))),
+        free_ports ip ports)%I -∗
+     frag_st Mdl.(model_state_initial) -∗
+     ([∗ set] lbl ∈ lbls, alloc_evs lbl []) -∗
+     ([∗ set] sa ∈ obs_send_sas, sendon_evs sa []) -∗
+     ([∗ set] sa ∈ obs_rec_sas, receiveon_evs sa []) -∗
+     observed_send obs_send_sas -∗
+     observed_receive obs_rec_sas -∗
+     aneris_state_interp σ (∅,∅) ={⊤}=∗
+     aneris_state_interp σ (∅,∅) ∗
+     aneris_wptp es ((λ φ, (λ v, ⌜φ v⌝):val → iProp Σ) <$> φs)) →
+  obs_send_sas ⊆ A → obs_rec_sas ⊆ A →
+  dom $ state_heaps σ = get_ips es →
+  dom $ state_sockets σ = get_ips es →
+  (* Port coherence *)
+  ((∀ ip ps, (GSet <$> (addrs_to_ip_ports_map
+                              (A ∖ (ports_in_use $ state_sockets σ))))
+               !! ip = Some (GSet ps) →
+             ∀ Sn, (state_sockets σ) !! ip = Some Sn →
+                   ∀ p, p ∈ ps → port_not_in_use p Sn)) →
+  (* Socket buffers are initially empty *)
+  map_Forall (λ ip s, map_Forall (λ sh sb, sb.2 = []) s) (state_sockets σ) →
+  map_Forall (λ ip s, socket_handlers_coh s) (state_sockets σ) →
+  map_Forall (λ ip s, socket_addresses_coh s ip) (state_sockets σ) →
+  (* Message soup is initially empty *)
+  state_ms σ = ∅ →
+  aneris_adequate_multiple es σ φs.
+Proof.
+  intros Hlen HMdlfin Hwp Hsendle Hrecvle Hσ Hskts Hports Hbs Hcoh1 Hcoh2 Hms.
+  rewrite /aneris_adequate_multiple.
+  rewrite /aneris_adequate_multiple. simpl.
+  eapply (adequacy_multiple_strong A _ obs_send_sas obs_rec_sas);
+    [done|done|done|done| |done..].
+  intros dg.
+  iMod (Hwp dg) as "Hwp".
+  iModIntro. iIntros "????? #Hns ?????? /=".
+  iSpecialize ("Hwp" with "[$] [$] [$] [$] [$] [$] [$] [$] [$] [$] [$]").
+  iMod "Hwp" as "[$ Hwp]". iModIntro. clear Hwp Hlen Hσ Hskts.
+  setoid_rewrite aneris_wp_unfold. rewrite /aneris_wp_def.
+  assert (∃ es', [] = es') as [es' ->] by eauto.
+  iDestruct (big_sepL_prefixes_l _ es' with "Hwp") as "Hwp".
+  iInduction es as [|e es] "IHes" forall (φs es'); [done|].
+  destruct φs; [done|].
+  rewrite /get_ips.
+  simpl.
+  iDestruct "Hwp" as "[Hwp Hwps]".
+  iDestruct (big_sepS_elem_of _ _ (expr_n e) with "Hns") as "Hn";
+    [set_solver|].
+  iSplitL "Hwp Hn".
+  { rewrite /locale_of. simpl.
+    destruct e; simpl.
+    iSpecialize ("Hwp" with "[$]").
+    iApply (wp_wand with "Hwp"). by eauto. }
+  iDestruct (big_sepS_subseteq _ _ (list_to_set
+                            (list_fmap aneris_expr ip_address expr_n es)) with "Hns") as "Hns'"; [set_solver|].
+  iDestruct ("IHes" with "Hns' Hwps") as "Hwps".
+  iApply (big_sepL2_impl with "Hwps").
+  by iIntros "!>" (i eφs1 eφs2 HSome1 HSome2) "Hwp".
+Qed.
+
+Theorem adequacy_multiple Σ Mdl `{anerisPreG Σ Mdl} `{EqDecision (aneris_to_trace_model Mdl)}
+        A lbls obs_send_sas obs_rec_sas (es : list aneris_expr) σ (φs : list (val → Prop)) :
+  length es >= 1 →
+  aneris_model_rel_finitary Mdl →
+  (∀ (aG : anerisG Mdl Σ), ⊢ |={⊤}=>
+     unallocated A -∗
+     ([∗ set] sa ∈ A, sa ⤳[bool_decide (sa ∈ obs_send_sas),
+                           bool_decide (sa ∈ obs_rec_sas)] (∅, ∅)) -∗
+     ([∗ map] ip ↦ ports ∈ addrs_to_ip_ports_map A, free_ports ip ports)%I -∗
+     frag_st Mdl.(model_state_initial) -∗
+     ([∗ set] lbl ∈ lbls, alloc_evs lbl []) -∗
+     ([∗ set] sa ∈ obs_send_sas, sendon_evs sa []) -∗
+     ([∗ set] sa ∈ obs_rec_sas, receiveon_evs sa []) -∗
+     observed_send obs_send_sas -∗
+     observed_receive obs_rec_sas -∗
+     aneris_state_interp σ (∅,∅) ={⊤}=∗
+     aneris_state_interp σ (∅,∅) ∗
+     aneris_wptp es ((λ φ, (λ v, ⌜φ v⌝):val → iProp Σ) <$> φs)) →
+  obs_send_sas ⊆ A → obs_rec_sas ⊆ A →
+  state_heaps σ = gset_to_gmap ∅ $ get_ips es →
+  state_sockets σ = gset_to_gmap ∅ $ get_ips es →
+  state_ms σ = ∅ →
+  aneris_adequate_multiple es σ φs.
+Proof.
+  intros Hlen HMdlfin Hwp Hsendle Hrecvle Hσ Hskts Hms.
+  eapply (adequacy_multiple A _ obs_send_sas obs_rec_sas);
+    [done|done|done|done| |done..].
+  intros dg.
+  iMod (Hwp dg) as "Hwp".
+  iModIntro. iIntros "???? #Hns ?????? /=".
+  iSpecialize ("Hwp" with "[$] [$] [$] [$] [$] [$] [$] [$] [$] [$]").
+  iMod "Hwp" as "[$ Hwp]". iModIntro. clear Hwp Hlen Hσ Hskts.
+  setoid_rewrite aneris_wp_unfold. rewrite /aneris_wp_def.
+  assert (∃ es', [] = es') as [es' ->] by eauto.
+  iDestruct (big_sepL_prefixes_l _ es' with "Hwp") as "Hwp".
+  iInduction es as [|e es] "IHes" forall (φs es'); [done|].
+  destruct φs; [done|].
+  rewrite /get_ips.
+  simpl.
+  iDestruct "Hwp" as "[Hwp Hwps]".
+  iDestruct (big_sepS_elem_of _ _ (expr_n e) with "Hns") as "Hn";
+    [set_solver|].
+  iSplitL "Hwp Hn".
+  { rewrite /locale_of. simpl.
+    destruct e; simpl.
+    iSpecialize ("Hwp" with "[$]").
+    iApply (wp_wand with "Hwp"). by eauto. }
+  iDestruct (big_sepS_subseteq _ _ (list_to_set
+                            (list_fmap aneris_expr ip_address expr_n es)) with "Hns") as "Hns'"; [set_solver|].
+  iDestruct ("IHes" with "Hns' Hwps") as "Hwps".
+  iApply (big_sepL2_impl with "Hwps").
+  by iIntros "!>" (i eφs1 eφs2 HSome1 HSome2) "Hwp".
+Qed.
 
 Definition aneris_adequate (e :expr) (ip : ip_address) (σ : state)
            (φ : val → Prop) :=
